lib_bitmap/Bitmap1.fst
@@ -266,6 +266,7 @@ let logand_one_sub (#n: pos) (a:uint_t n) (b:uint_t n) (m:nat{m < n})
   assert (from_vec vb = b);
   assert (r = b - 1 * a)
 #pop-options
+
 let spec_bv_unset (#n:pos) (b:uint_t n) (m:nat{m < n})
   : Lemma
   (requires
